lib/parseTreeScript.sml
@@ -2,9 +2,9 @@
 open HolKernel boolLib bossLib Parse Defn BasicProvers
 
 open stringTheory grammarDefTheory symbolDefTheory listTheory pairTheory
-optionTheory
+optionTheory rich_listTheory pred_setTheory
 
-open listLemmasTheory
+open listLemmasTheory containerLemmasTheory
 
 val _ = new_theory "parseTree";
 
@@ -323,6 +323,473 @@ val fringeEqLeaves = store_thm
 HO_MATCH_MP_TAC fringe_ind THEN SRW_TAC [][] THEN
 SRW_TAC [][fringe_def, leaves_def] THEN
 METIS_TAC [mapFringeLeaves]);
+
+val treeSyms_defn = Hol_defn "treeSyms_defn"
+`(treeSyms (Leaf tm) =  ([TS tm]:(α,β) symbol list)) ∧
+(treeSyms (Node n t) =  (NTS n) :: (FLAT (MAP treeSyms t)))`;
+
+val (treeSyms, treeSyms_ind) = tprove (treeSyms_defn,
+WF_REL_TAC (`measure ptsize`) THEN
+SRW_TAC [] [] THEN
+FULL_SIMP_TAC (srw_ss()) [rgr_r9eq, ptsizel_append] THEN
+DECIDE_TAC);
+
+val _ = save_thm ("treeSyms_def",treeSyms)
+val _ = save_thm ("treeSyms_ind",treeSyms_ind)
+
+
+val distinctNtms = Define
+`distinctNtms t = rmDupes (FILTER isNonTmnlSym (treeSyms t))`;
+
+val subtree = Define
+`(subtree (Leaf tm) (p::ps) = NONE) ∧
+(subtree t [] = SOME t) ∧
+(subtree (Node n ptl) (p::ps) = 
+ if (p < LENGTH ptl) then
+     subtree (EL p ptl) ps else NONE)`;
+
+val subtPathNil = store_thm
+("subtPathNil",
+``(subtree t [] = SOME t1) ⇔ (t = t1)``,
+
+Cases_on `t` THEN SRW_TAC [][subtree]);
+
+val _ = export_rewrites ["subtPathNil"];
+
+
+val isSubtree = Define
+`isSubtree st t = ∃p. p ≠ [] ∧ (subtree t p = SOME st)`;
+
+val isSubtreeEq = Define
+`isSubtreeEq st t =  ∃p.(subtree t p = SOME st)`;
+
+val allTms = Define
+`allTms ptl = isWord (MAP root ptl)`;
+
+val btree = Define
+`btree B st t = (root st = B) ∧  isSubtree st t`;
+
+val subtreeApp = store_thm
+("subtreeApp",
+``∀t t1 p p'.
+ (subtree t p = SOME t1) ∧ (subtree t1 p' = SOME t0) ⇒
+ (subtree t (p++p') = SOME t0)``,
+
+Induct_on `p` THEN SRW_TAC [][] THEN
+Cases_on `t` THEN
+FULL_SIMP_TAC (srw_ss()) [subtree] THEN
+Cases_on `h < LENGTH l` THEN FULL_SIMP_TAC (srw_ss()) []);
+
+
+val subtreeTrans = store_thm 
+("subtreeTrans",
+``∀t0 t1 t. isSubtree t1 t ∧ isSubtree t0 t1 ⇒ isSubtree t0 t``,
+
+FULL_SIMP_TAC (srw_ss()) [isSubtree] THEN
+SRW_TAC [][] THEN
+Q.EXISTS_TAC `p ++ p'` THEN
+SRW_TAC [][] THEN
+METIS_TAC [subtreeApp]);
+
+
+val subtreeEqTrans = store_thm 
+("subtreeEqTrans",
+``∀t0 t1 t. isSubtreeEq t1 t ∧ isSubtreeEq t0 t1 ⇒ isSubtreeEq t0 t``,
+
+FULL_SIMP_TAC (srw_ss()) [isSubtreeEq] THEN
+SRW_TAC [][] THEN
+Q.EXISTS_TAC `p ++ p'` THEN
+SRW_TAC [][] THEN
+METIS_TAC [subtreeApp]);
+
+val subtImpisSubt = store_thm
+("subtImpisSubt",
+``∀t p t1. (subtree t p = SOME t1) ∧ p ≠ [] ⇒ isSubtree t1 t``,
+
+Induct_on `p` THEN SRW_TAC [][subtree] THEN
+Cases_on `t` THEN FULL_SIMP_TAC (srw_ss()) [subtree, isSubtree] THEN
+Cases_on `h < LENGTH l` THEN FULL_SIMP_TAC (srw_ss())[] THEN
+Cases_on `p` THEN FULL_SIMP_TAC (srw_ss()) [subtree] THEN1
+(Cases_on `EL h l` THEN FULL_SIMP_TAC (srw_ss()) [subtree] THEN
+ SRW_TAC [][] THEN
+ Q.EXISTS_TAC `[h]` THEN
+ SRW_TAC [][subtree]) THEN
+
+FIRST_X_ASSUM (Q.SPECL_THEN [`EL h l`, `t1`] MP_TAC) THEN SRW_TAC [][] THEN
+Q.EXISTS_TAC `h::h'::t` THEN
+SRW_TAC [][subtree]);
+
+
+val isSubEqImpSub = store_thm
+("isSubEqImpSub",
+``isSubtreeEq t1 t ⇔ (t1 = t) ∨ isSubtree t1 t``,
+
+SRW_TAC [][isSubtree, isSubtreeEq, EQ_IMP_THM] THEN1
+
+(Cases_on `t` THEN Cases_on `p` THEN FULL_SIMP_TAC (srw_ss()) [subtree] THEN
+Cases_on `h < LENGTH l` THEN FULL_SIMP_TAC (srw_ss()) [] THEN
+DISJ2_TAC THEN
+Q.EXISTS_TAC `h::t` THEN
+SRW_TAC [][subtree]) THEN1
+
+(Cases_on `t` THEN METIS_TAC [subtree]) THEN
+
+METIS_TAC []);
+
+ 
+
+val subtreeHeight = store_thm
+("subtreeHeight",
+``∀t p t1. (subtree t p = SOME t1) ∧ p ≠ [] ⇒ height t1 < height t``,
+
+Induct_on `p` THEN SRW_TAC [][] THEN
+Cases_on `t` THEN
+FULL_SIMP_TAC (srw_ss()) [subtree] THEN
+Cases_on `h < LENGTH l` THEN FULL_SIMP_TAC (srw_ss()) [] THEN
+FIRST_X_ASSUM (Q.SPECL_THEN [`EL h l`, `t1`] MP_TAC) THEN
+SRW_TAC [][] THEN
+Cases_on `p` THEN FULL_SIMP_TAC (srw_ss()) [] THEN1
+
+(Cases_on `EL h l` THEN
+FULL_SIMP_TAC (srw_ss()) [subtree, height_def] THEN
+SRW_TAC [][height_def] THEN
+`MEM (EL h l) l` by METIS_TAC [EL_IS_EL] THEN
+FULL_SIMP_TAC (srw_ss()) [rgr_r9eq] THEN SRW_TAC [][] THEN
+FULL_SIMP_TAC (srw_ss()) [] THEN
+ONCE_ASM_REWRITE_TAC [] THEN
+ONCE_ASM_REWRITE_TAC [] THEN
+SRW_TAC [][height_def] THEN1
+DECIDE_TAC  THEN
+Q.ABBREV_TAC `n = max 0 (MAP (λa. height a) l')` THEN
+METIS_TAC [maxGtElem, MEM, MEM_APPEND, DECIDE ``1 + n > n``]) THEN
+
+SRW_TAC [][height_def] THEN
+`MEM (EL h l) l` by METIS_TAC [EL_IS_EL] THEN
+FULL_SIMP_TAC (srw_ss()) [rgr_r9eq] THEN SRW_TAC [][] THEN
+FULL_SIMP_TAC (srw_ss()) [] THEN
+ONCE_ASM_REWRITE_TAC [] THEN
+SRW_TAC [][height_def] THEN
+`height (EL h l) > height t1` by DECIDE_TAC THEN
+METIS_TAC [maxGtElem, MEM, MEM_APPEND, DECIDE ``a < b ⇒ a < 1 + b``]);
+
+val treeSymsImpSubtree = store_thm
+("treeSymsImpSubtree",
+``∀t. e ∈ treeSyms t ⇒ ∃t1. isSubtreeEq t1 t ∧ (root t1 = e)``,
+
+completeInduct_on `height t` THEN SRW_TAC [][] THEN
+Cases_on `t` THEN FULL_SIMP_TAC (srw_ss()) [height_def, treeSyms] THEN1
+(SRW_TAC [][isSubtreeEq] THEN
+Q.EXISTS_TAC `Leaf t'` THEN
+SRW_TAC [][root] THEN
+Q.EXISTS_TAC `[]` THEN SRW_TAC [][subtree]) THEN1
+(SRW_TAC [][] THEN
+Q.EXISTS_TAC `Node n l` THEN
+SRW_TAC [][root, isSubtreeEq] THEN
+Q.EXISTS_TAC `[]` THEN SRW_TAC [][subtree]) THEN
+
+FULL_SIMP_TAC (srw_ss()) [MEM_FLAT, MEM_MAP] THEN
+SRW_TAC [][] THEN
+`isSubtree a (Node n l)` by
+(IMP_RES_TAC memImpEl THEN
+SRW_TAC [][isSubtree] THEN
+Q.EXISTS_TAC `[i']` THEN
+SRW_TAC [][subtree] THEN
+Cases_on `EL i' l`THEN SRW_TAC [][subtree]) THEN
+`height a < 1 + max 0 (MAP (λa. height a) l)` by
+(`height a < height (Node n l)`by METIS_TAC [subtreeHeight, isSubtree] THEN
+FULL_SIMP_TAC (srw_ss()) [height_def]) THEN
+METIS_TAC [subtreeTrans, isSubtree, isSubEqImpSub]);
+
+val numd = store_thm
+("numd",
+ ``∀t. isNode t ⇒ LENGTH (distinctNtms t) ≥ 1``,
+
+Cases_on `t` THEN SRW_TAC [][distinctNtms, treeSyms, rmDupes, delete_def,isNode,
+			     rmDupes, FILTER_APPEND, isNonTmnlSym_def] THEN
+DECIDE_TAC);
+
+val subtreeLevel = store_thm
+("subtreeLevel",
+``∀t p. (subtree t p = SOME t1) ∧ p ≠ [] ⇒
+   ∃n ptl. (subtree t (FRONT p) = SOME (Node n ptl)) ∧ MEM t1 ptl``,
+
+Induct_on `p` THEN SRW_TAC [][] THEN
+Cases_on `t` THEN FULL_SIMP_TAC (srw_ss()) [subtree] THEN
+Cases_on `h < LENGTH l` THEN FULL_SIMP_TAC (srw_ss()) [] THEN
+Cases_on `p` THEN FULL_SIMP_TAC (srw_ss()) [] THEN1
+
+(Cases_on `EL h l` THEN
+FULL_SIMP_TAC (srw_ss()) [subtree] THEN
+SRW_TAC [][] THEN
+METIS_TAC [EL_IS_EL]) THEN
+SRW_TAC [][subtree]);
+
+val distNtmsSub = store_thm
+("distNtmsSub",
+``∀g t. validptree g t ⇒ set (distinctNtms t) ⊆  set (MAP NTS (ntms g))``,
+
+HO_MATCH_MP_TAC validptree_ind THEN
+SRW_TAC [][validptree] THEN
+`∀e. e ∈ ptl ∧ isNode e ⇒ set (distinctNtms e) ⊆ set (MAP NTS (ntms g))`
+by METIS_TAC [] THEN
+`∀e. e ∈ ptl ⇒ set (distinctNtms e) ⊆ set (MAP NTS (ntms g))` by
+(SRW_TAC [][] THEN
+Cases_on `e` THEN1
+SRW_TAC [][distinctNtms, isNonTmnlSym_def, treeSyms, rmDupes, delete_def] THEN
+METIS_TAC [isNode]) THEN
+`n ∈ (ntms g)`  by METIS_TAC [ruleRhsInntms] THEN
+`((NTS n):(α,β) symbol) ∈ (MAP NTS (ntms g))`  by SRW_TAC [][MEM_MAP] THEN
+FULL_SIMP_TAC (srw_ss()) [distinctNtms, treeSyms, isNonTmnlSym_def,
+			  SUBSET_DEF, EXTENSION] THEN
+SRW_TAC [][] THEN
+FULL_SIMP_TAC (srw_ss())[rmDupes] THEN
+`x ∈ (FILTER isNonTmnlSym (FLAT (MAP (λa. treeSyms a) ptl)))`
+ by METIS_TAC [memdel, rmd_r2] THEN
+FULL_SIMP_TAC (srw_ss()) [MEM_FILTER, MEM_MAP, MEM_FLAT] THEN
+SRW_TAC [][] THEN
+`x ∈ FILTER isNonTmnlSym (treeSyms a)` by METIS_TAC [MEM_FILTER] THEN
+Cases_on `x` THEN FULL_SIMP_TAC (srw_ss()) [isNonTmnlSym_def] THEN
+METIS_TAC [rmd_r2, symbol_11]);
+
+
+val LENGTH_distinctNtms = store_thm(
+  "LENGTH_distinctNtms",
+  ``LENGTH (distinctNtms t) = CARD (set (distinctNtms t))``,
+  SRW_TAC [][distinctNtms, rmDupes_lts_card, rmDupes_lts_card_eq]);
+
+val LENGTH_ntms = store_thm(
+  "LENGTH_ntms",
+  ``LENGTH (ntms t) = CARD (set (ntms t))``,
+  SRW_TAC [][ntms_def, rmDupes_lts_card, rmDupes_lts_card_eq]);
+
+
+val numdLeqNtms = store_thm
+("numdLeqNtms",
+``∀g t. validptree g t ⇒ LENGTH (distinctNtms t) ≤ LENGTH (ntms g)``,
+
+SRW_TAC [][] THEN
+Q_TAC SUFF_TAC ` LENGTH (distinctNtms t) ≤ 
+ LENGTH ((MAP NTS (ntms g)):(α,β) symbol list)` THEN1
+ METIS_TAC [LENGTH_MAP] THEN
+IMP_RES_TAC distNtmsSub THEN
+`FINITE (set (distinctNtms t))` by METIS_TAC [FINITE_LIST_TO_SET] THEN
+SRW_TAC [][LENGTH_ntms, LENGTH_distinctNtms] THEN
+`∀x y.(NTS x = NTS y) ⇔ (x = y)` by FULL_SIMP_TAC (srw_ss()) [] THEN
+`CARD (set ((MAP NTS (ntms g)):(α,β) symbol list)) =
+CARD (set (ntms g))` by METIS_TAC [mapCard, FINITE_LIST_TO_SET] THEN
+METIS_TAC [CARD_SUBSET, FINITE_LIST_TO_SET, DECIDE ``a ≤ b ∧b ≤ c ⇒ a ≤ c``]);
+
+
+val cleavesApp = store_thm
+("cleavesApp",
+``∀a b. cleaves (a ++ b) = cleaves a ++ cleaves b``,
+
+Induct_on `a` THEN SRW_TAC [][leaves_def]);
+
+
+val subtreePfxSfxLeaves = store_thm
+("subtreePfxSfxLeaves",
+``∀t t1 p.(subtree t p = SOME t1) ⇒ 
+∃pfx sfx.(leaves t = pfx ++ leaves t1 ++ sfx)``,
+
+Induct_on `p` THEN SRW_TAC [][] THEN1
+
+(Cases_on `t` THEN FULL_SIMP_TAC (srw_ss()) [subtree] THEN
+ METIS_TAC [APPEND_NIL]) THEN
+
+Cases_on `t` THEN
+FULL_SIMP_TAC (srw_ss()) [] THEN1
+FULL_SIMP_TAC (srw_ss()) [subtree] THEN
+FULL_SIMP_TAC (srw_ss()) [subtree] THEN
+Cases_on `h < LENGTH l` THEN FULL_SIMP_TAC (srw_ss()) [] THEN
+FIRST_X_ASSUM (Q.SPECL_THEN [`EL h l`,`t1`] MP_TAC) THEN SRW_TAC [][] THEN
+
+(Cases_on `EL h l` THEN
+FULL_SIMP_TAC (srw_ss()) [subtree, leaves_def] THEN
+SRW_TAC [][leaves_def] THEN
+`MEM (EL h l) l` by METIS_TAC [EL_IS_EL] THEN
+FULL_SIMP_TAC (srw_ss()) [rgr_r9eq] THEN
+ONCE_ASM_REWRITE_TAC [] THEN
+SRW_TAC [][cleavesApp, leaves_def] THEN
+METIS_TAC [APPEND_ASSOC]));
+
+val vptSubtree = store_thm
+("vptSubtree",
+``∀g t. validptree g t ⇒ 
+ (∀t1. isSubtreeEq t1 t ∧ isNode t1 ⇒ validptree g t1)``,
+
+completeInduct_on `height t` THEN SRW_TAC [][] THEN
+Cases_on `t` THEN FULL_SIMP_TAC (srw_ss()) [] THEN1
+FULL_SIMP_TAC (srw_ss()) [validptree] THEN
+FULL_SIMP_TAC (srw_ss()) [isSubEqImpSub, isSubtree] THEN
+
+Cases_on `p` THEN FULL_SIMP_TAC (srw_ss()) [subtree] THEN
+Cases_on `h < LENGTH l` THEN FULL_SIMP_TAC (srw_ss()) [] THEN
+`isSubtreeEq t1 (EL h l)` by
+(SRW_TAC [][isSubEqImpSub, isSubtree] THEN
+Cases_on `t` THEN FULL_SIMP_TAC (srw_ss()) [subtree] THEN
+METIS_TAC [MEM]) THEN
+`isSubtree (EL h l) (Node n l)` by
+(SRW_TAC [][isSubtree] THEN
+Q.EXISTS_TAC `[h]` THEN SRW_TAC [][subtree] THEN
+Cases_on `EL h l` THEN SRW_TAC [][subtree]) THEN
+Cases_on `EL h l` THEN1
+(Cases_on `t` THEN FULL_SIMP_TAC (srw_ss()) [validptree, subtree] THEN
+Cases_on `t1` THEN FULL_SIMP_TAC (srw_ss()) [isNode]) THEN
+`height (EL h l) < height (Node n l)` by METIS_TAC [isSubtree, subtreeHeight] THEN
+FIRST_X_ASSUM (Q.SPECL_THEN [`height (EL h l)`] MP_TAC) THEN SRW_TAC [][] THEN
+FIRST_X_ASSUM (Q.SPECL_THEN [`EL h l`] MP_TAC) THEN SRW_TAC [][] THEN
+`validptree g (Node n' l')` by
+(FULL_SIMP_TAC (srw_ss()) [validptree] THEN
+METIS_TAC [isNode, EL_IS_EL, validptree]) THEN
+FIRST_X_ASSUM (Q.SPECL_THEN [`g`] MP_TAC) THEN SRW_TAC [][] THEN
+
+FULL_SIMP_TAC (srw_ss()) [isSubEqImpSub, isSubtree] THEN
+METIS_TAC []);
+
+
+
+val leafSubt = store_thm
+("leafSubt",
+``isSubtree t0 (Node n [Leaf ts]) ⇒ (t0 = Leaf ts)``,
+
+SRW_TAC [][isSubtree] THEN
+Cases_on `p` THEN FULL_SIMP_TAC (srw_ss()) [subtree] THEN
+Cases_on `h < 1` THEN FULL_SIMP_TAC (srw_ss()) [] THEN
+`h = 0` by DECIDE_TAC THEN
+SRW_TAC [][] THEN
+FULL_SIMP_TAC (srw_ss()) [] THEN
+Cases_on `t` THEN FULL_SIMP_TAC (srw_ss()) [subtree]);
+
+
+val subtDistNtms = store_thm
+("subtDistNtms",
+``∀t t1 p. (subtree t p = SOME t1) ⇒ 
+LENGTH (distinctNtms t1) ≤ LENGTH (distinctNtms t)``,
+
+Induct_on `p` THEN SRW_TAC [][] THEN
+Cases_on `t` THEN
+FULL_SIMP_TAC (srw_ss()) [subtree] THEN
+Cases_on `h < LENGTH l` THEN FULL_SIMP_TAC (srw_ss()) [] THEN
+FIRST_X_ASSUM (Q.SPECL_THEN [`EL h l`,`t1`] MP_TAC) THEN SRW_TAC [][] THEN
+
+`LENGTH (distinctNtms (EL h l)) ≤ LENGTH (distinctNtms (Node n l))`
+by (SRW_TAC [][distinctNtms, treeSyms] THEN
+`(EL h l) ∈ l`by METIS_TAC [EL_IS_EL] THEN
+FULL_SIMP_TAC (srw_ss()) [rgr_r9eq, isNonTmnlSym_def] THEN
+SRW_TAC [][] THEN
+Q_TAC SUFF_TAC `LENGTH (rmDupes (FILTER isNonTmnlSym (treeSyms (EL h l)))) ≤
+LENGTH
+  (rmDupes
+     (NTS n::
+          FILTER isNonTmnlSym
+            (FLAT (MAP (λa. treeSyms a) (r1 ++ [EL h l] ++ r2)))))` THEN1
+METIS_TAC [] THEN
+SRW_TAC [][FILTER_APPEND, FLAT_APPEND] THEN
+METIS_TAC [rmdLenLe, APPEND, APPEND_ASSOC]) THEN
+DECIDE_TAC);
+
+
+
+val distSymsLenSub = store_thm
+("distSymsLenSub",
+``∀t1 t. isSubtreeEq t1 t ⇒ LENGTH (distinctNtms t1) ≤ LENGTH (distinctNtms t)``,
+
+SRW_TAC [][isSubtreeEq] THEN
+METIS_TAC [subtDistNtms]);
+
+
+
+val cnfTree = store_thm
+("cnfTree",
+``∀g tree. validptree g tree ⇒ isCnf g ⇒ ∀n t. (tree = Node n t) ⇒
+    ∃n1 t1 n2 t2.(t = [Node n1 t1; Node n2 t2]) ∨ ∃ts.(t = [Leaf ts])``,
+
+HO_MATCH_MP_TAC validptree_ind THEN SRW_TAC [][] THEN
+FULL_SIMP_TAC (srw_ss()) [validptree, isCnf_def] THEN
+RES_TAC THEN
+FULL_SIMP_TAC (srw_ss()) [list_lem2, list_lem1] THEN1
+(Cases_on `e1` THEN Cases_on `e2` THEN
+ SRW_TAC [][] THEN
+ FULL_SIMP_TAC (srw_ss()) [isNonTmnlSym_def, isNode] THEN1
+(`∃t1 t2.ptl = [Node n' t1; Node n'' t2]` by METIS_TAC [getSymsNtm] THEN
+METIS_TAC []) THEN
+(RES_TAC THEN
+FULL_SIMP_TAC (srw_ss()) [] THEN SRW_TAC [][] THEN
+FULL_SIMP_TAC (srw_ss()) [isNonTmnlSym_def])) THEN
+FULL_SIMP_TAC (srw_ss()) [] THEN
+RES_TAC THEN
+FULL_SIMP_TAC (srw_ss()) [] THEN SRW_TAC [][] THEN
+Cases_on `e` THEN FULL_SIMP_TAC (srw_ss()) [isTmnlSym_def] THEN
+`ptl = [Leaf t]` by METIS_TAC [getSymsTm] THEN
+METIS_TAC []);
+
+val cnfTreeLeaves = store_thm
+("cnfTreeLeaves",
+``∀g t. validptree g t ⇒ isCnf g ⇒ LENGTH (leaves t) ≥ 1``,
+
+HO_MATCH_MP_TAC validptree_ind THEN SRW_TAC [][] THEN
+FULL_SIMP_TAC (srw_ss()) [validptree, isCnf_def] THEN
+Q.ABBREV_TAC `r = getSymbols ptl` THEN
+`EVERY isNonTmnlSym r ∧ (LENGTH r = 2) ∨
+isWord r ∧ (LENGTH r = 1)` by METIS_TAC [] THEN
+SRW_TAC [][] THEN
+FULL_SIMP_TAC (srw_ss()) [list_lem2, list_lem1] THEN1
+(Cases_on `e1` THEN Cases_on `e2` THEN
+ SRW_TAC [][] THEN
+ FULL_SIMP_TAC (srw_ss()) [isNonTmnlSym_def, isNode] THEN
+`∃t1 t2.ptl = [Node n' t1; Node n'' t2]` by METIS_TAC [getSymsNtm] THEN
+SRW_TAC [][leaves_def] THEN
+FULL_SIMP_TAC (srw_ss()) [] THEN
+`LENGTH (leaves (Node n' t1)) ≥ 1`by METIS_TAC [isNode] THEN
+`LENGTH (leaves (Node n'' t2)) ≥ 1`by METIS_TAC [isNode] THEN
+FULL_SIMP_TAC (srw_ss()++ARITH_ss) [leaves_def]) THEN
+Cases_on `e` THEN
+SRW_TAC [][] THEN FULL_SIMP_TAC (srw_ss()) [isTmnlSym_def] THEN
+`(ptl = [Leaf t])` by METIS_TAC [getSymsTm] THEN
+SRW_TAC [][leaves_def]);
+
+
+val rootRep = Define
+`rootRep st t = (root st = root t) ∧  isSubtree st t`;
+
+
+val symRepProp = Define
+`symRepProp t0 t1 t = isSubtreeEq t1 t ∧ rootRep t0 t1`;
+
+val subtreeNotSymProp = store_thm
+("subtreeNotSymProp",
+``(subtree t p = SOME t1) ∧ (¬∃s0 s1. symRepProp s0 s1 t) ⇒
+ ¬∃s0 s1. symRepProp s0 s1 t1``,
+
+SRW_TAC [][symRepProp] THEN
+SPOSE_NOT_THEN ASSUME_TAC THEN 
+FULL_SIMP_TAC (srw_ss()) [btree] THEN
+`isSubtreeEq t1 t` by METIS_TAC [isSubtreeEq, option_CLAUSES] THEN
+METIS_TAC [subtreeEqTrans,root, isSubtree, root, isSubtreeEq]);
+
+
+val notSymRepImpTreeSyms = store_thm
+("notSymRepImpTreeSyms",
+``(∀t0 t1. ¬symRepProp t0 t1 (Node n ptl)) ⇒ 
+(∀e. e ∈ ptl ⇒ ¬((NTS n) ∈ treeSyms e))``,
+
+SRW_TAC [][] THEN
+SPOSE_NOT_THEN ASSUME_TAC THEN
+IMP_RES_TAC treeSymsImpSubtree THEN
+`isSubtree e (Node n ptl)` by
+(IMP_RES_TAC memImpEl THEN
+SRW_TAC [][isSubtree] THEN
+Q.EXISTS_TAC `[i']` THEN
+SRW_TAC [][subtree] THEN
+Cases_on `EL i' ptl` THEN SRW_TAC [][subtree]) THEN
+
+`symRepProp t1 (Node n ptl) (Node n ptl)` by
+(FULL_SIMP_TAC (srw_ss()) [symRepProp, isSubEqImpSub, rootRep, root] THEN
+METIS_TAC [isSubtree, subtreeTrans]) THEN
+METIS_TAC []);
+
+
 
 
 val mlDir = ref ("./theoryML/");
