pda/pumpingLemmaTreeScript.sml
@@ -14,53 +14,6 @@ val _ = Globals.linewidth := 60
 val _ = set_trace "Unicode" 1
 
 
-val treeSyms_defn = Hol_defn "treeSyms_defn"
-`(treeSyms (Leaf tm) =  ([TS tm]:(α,β) symbol list)) ∧
-(treeSyms (Node n t) =  (NTS n) :: (FLAT (MAP treeSyms t)))`;
-
-val (treeSyms, treeSyms_ind) = tprove (treeSyms_defn,
-WF_REL_TAC (`measure ptsize`) THEN
-SRW_TAC [] [] THEN
-FULL_SIMP_TAC (srw_ss()) [rgr_r9eq, ptsizel_append] THEN
-DECIDE_TAC);
-
-val distinctNtms = Define
-`distinctNtms t = rmDupes (FILTER isNonTmnlSym (treeSyms t))`;
-
-val subtree = Define
-`(subtree (Leaf tm) (p::ps) = NONE) ∧
-(subtree t [] = SOME t) ∧
-(subtree (Node n ptl) (p::ps) = 
- if (p < LENGTH ptl) then
-     subtree (EL p ptl) ps else NONE)`;
-
-val subtPathNil = store_thm
-("subtPathNil",
-``(subtree t [] = SOME t1) ⇔ (t = t1)``,
-
-Cases_on `t` THEN SRW_TAC [][subtree]);
-
-val _ = export_rewrites ["subtPathNil"];
-
-
-val isSubtree = Define
-`isSubtree st t = ∃p. p ≠ [] ∧ (subtree t p = SOME st)`;
-
-val isSubtreeEq = Define
-`isSubtreeEq st t =  ∃p.(subtree t p = SOME st)`;
-
-val allTms = Define
-`allTms ptl = isWord (MAP root ptl)`;
-
-val btree = Define
-`btree B st t = (root st = B) ∧  isSubtree st t`;
-
-val rootRep = Define
-`rootRep st t = (root st = root t) ∧  isSubtree st t`;
-
-
-val symRepProp = Define
-`symRepProp t0 t1 t = isSubtreeEq t1 t ∧ rootRep t0 t1`;
 
 
 val lastExpProp = Define
@@ -71,94 +24,13 @@ val lastExpProp = Define
 
 
 
-val subtreeApp = store_thm
-("subtreeApp",
-``∀t t1 p p'.
- (subtree t p = SOME t1) ∧ (subtree t1 p' = SOME t0) ⇒
- (subtree t (p++p') = SOME t0)``,
-
-Induct_on `p` THEN SRW_TAC [][] THEN
-Cases_on `t` THEN
-FULL_SIMP_TAC (srw_ss()) [subtree] THEN
-Cases_on `h < LENGTH l` THEN FULL_SIMP_TAC (srw_ss()) []);
-
-
-val subtreeTrans = store_thm 
-("subtreeTrans",
-``∀t0 t1 t. isSubtree t1 t ∧ isSubtree t0 t1 ⇒ isSubtree t0 t``,
-
-FULL_SIMP_TAC (srw_ss()) [isSubtree] THEN
-SRW_TAC [][] THEN
-Q.EXISTS_TAC `p ++ p'` THEN
-SRW_TAC [][] THEN
-METIS_TAC [subtreeApp]);
-
-
-val subtreeEqTrans = store_thm 
-("subtreeEqTrans",
-``∀t0 t1 t. isSubtreeEq t1 t ∧ isSubtreeEq t0 t1 ⇒ isSubtreeEq t0 t``,
-
-FULL_SIMP_TAC (srw_ss()) [isSubtreeEq] THEN
-SRW_TAC [][] THEN
-Q.EXISTS_TAC `p ++ p'` THEN
-SRW_TAC [][] THEN
-METIS_TAC [subtreeApp]);
-
-val subtImpisSubt = store_thm
-("subtImpisSubt",
-``∀t p t1. (subtree t p = SOME t1) ∧ p ≠ [] ⇒ isSubtree t1 t``,
-
-Induct_on `p` THEN SRW_TAC [][subtree] THEN
-Cases_on `t` THEN FULL_SIMP_TAC (srw_ss()) [subtree, isSubtree] THEN
-Cases_on `h < LENGTH l` THEN FULL_SIMP_TAC (srw_ss())[] THEN
-Cases_on `p` THEN FULL_SIMP_TAC (srw_ss()) [subtree] THEN1
-(Cases_on `EL h l` THEN FULL_SIMP_TAC (srw_ss()) [subtree] THEN
- SRW_TAC [][] THEN
- Q.EXISTS_TAC `[h]` THEN
- SRW_TAC [][subtree]) THEN
-
-FIRST_X_ASSUM (Q.SPECL_THEN [`EL h l`, `t1`] MP_TAC) THEN SRW_TAC [][] THEN
-Q.EXISTS_TAC `h::h'::t` THEN
-SRW_TAC [][subtree]);
-
-
-val subtreeNotSymProp = store_thm
-("subtreeNotSymProp",
-``(subtree t p = SOME t1) ∧ (¬∃s0 s1. symRepProp s0 s1 t) ⇒
- ¬∃s0 s1. symRepProp s0 s1 t1``,
-
-SRW_TAC [][symRepProp] THEN
-SPOSE_NOT_THEN ASSUME_TAC THEN 
-FULL_SIMP_TAC (srw_ss()) [btree] THEN
-`isSubtreeEq t1 t` by METIS_TAC [isSubtreeEq, option_CLAUSES] THEN
-METIS_TAC [subtreeEqTrans,root_def, isSubtree, root_def, isSubtreeEq]);
-
-
-val isSubEqImpSub = store_thm
-("isSubEqImpSub",
-``isSubtreeEq t1 t ⇔ (t1 = t) ∨ isSubtree t1 t``,
-
-SRW_TAC [][isSubtree, isSubtreeEq, EQ_IMP_THM] THEN1
-
-(Cases_on `t` THEN Cases_on `p` THEN FULL_SIMP_TAC (srw_ss()) [subtree] THEN
-Cases_on `h < LENGTH l` THEN FULL_SIMP_TAC (srw_ss()) [] THEN
-DISJ2_TAC THEN
-Q.EXISTS_TAC `h::t` THEN
-SRW_TAC [][subtree]) THEN1
-
-(Cases_on `t` THEN METIS_TAC [subtree]) THEN
-
-METIS_TAC []);
-
- 
-
 val subtreeLastExp = store_thm
 ("subtreeLastExp",
 ``∀t t1. lastExpProp t1 ∧ isSubtree t1 t ⇒
  lastExpProp t``,
 
-SRW_TAC [][isSubtree, lastExpProp, isSubEqImpSub] THEN
-FULL_SIMP_TAC (srw_ss()) [symRepProp, btree] THEN
+SRW_TAC [][isSubtree_def, lastExpProp, isSubEqImpSub] THEN
+FULL_SIMP_TAC (srw_ss()) [symRepProp_def, btree_def] THEN
 
 FULL_SIMP_TAC (srw_ss()) [isSubEqImpSub] THEN
 SRW_TAC [][] THEN
@@ -166,42 +38,7 @@ SRW_TAC [][] THEN
 (MAP_EVERY Q.EXISTS_TAC [`t0`,`Node n ptl`] THEN
 FULL_SIMP_TAC (srw_ss()) [root_def] THEN
 SRW_TAC [][] THEN
-METIS_TAC [isSubtree, subtreeTrans, option_CLAUSES,root_def]));
-
-
-val subtreeHeight = store_thm
-("subtreeHeight",
-``∀t p t1. (subtree t p = SOME t1) ∧ p ≠ [] ⇒ height t1 < height t``,
-
-Induct_on `p` THEN SRW_TAC [][] THEN
-Cases_on `t` THEN
-FULL_SIMP_TAC (srw_ss()) [subtree] THEN
-Cases_on `h < LENGTH l` THEN FULL_SIMP_TAC (srw_ss()) [] THEN
-FIRST_X_ASSUM (Q.SPECL_THEN [`EL h l`, `t1`] MP_TAC) THEN
-SRW_TAC [][] THEN
-Cases_on `p` THEN FULL_SIMP_TAC (srw_ss()) [] THEN1
-
-(Cases_on `EL h l` THEN
-FULL_SIMP_TAC (srw_ss()) [subtree, height_def] THEN
-SRW_TAC [][height_def] THEN
-`MEM (EL h l) l` by METIS_TAC [EL_IS_EL] THEN
-FULL_SIMP_TAC (srw_ss()) [rgr_r9eq] THEN SRW_TAC [][] THEN
-FULL_SIMP_TAC (srw_ss()) [] THEN
-ONCE_ASM_REWRITE_TAC [] THEN
-ONCE_ASM_REWRITE_TAC [] THEN
-SRW_TAC [][height_def] THEN1
-DECIDE_TAC  THEN
-Q.ABBREV_TAC `n = max 0 (MAP (λa. height a) l')` THEN
-METIS_TAC [maxGtElem, MEM, MEM_APPEND, DECIDE ``1 + n > n``]) THEN
-
-SRW_TAC [][height_def] THEN
-`MEM (EL h l) l` by METIS_TAC [EL_IS_EL] THEN
-FULL_SIMP_TAC (srw_ss()) [rgr_r9eq] THEN SRW_TAC [][] THEN
-FULL_SIMP_TAC (srw_ss()) [] THEN
-ONCE_ASM_REWRITE_TAC [] THEN
-SRW_TAC [][height_def] THEN
-`height (EL h l) > height t1` by DECIDE_TAC THEN
-METIS_TAC [maxGtElem, MEM, MEM_APPEND, DECIDE ``a < b ⇒ a < 1 + b``]);
+METIS_TAC [isSubtree_def, subtreeTrans, option_CLAUSES,root_def]));
 
 
 val symPropImpLastExp = store_thm
@@ -211,26 +48,26 @@ val symPropImpLastExp = store_thm
 completeInduct_on `height t` THEN
 SRW_TAC [][] THEN
 Cases_on `t` THEN1
-(FULL_SIMP_TAC (srw_ss()) [lastExpProp, symRepProp, isSubtreeEq] THEN
- Cases_on `p` THEN FULL_SIMP_TAC (srw_ss()) [subtree] THEN
+(FULL_SIMP_TAC (srw_ss()) [lastExpProp, symRepProp_def, isSubtreeEq_def] THEN
+ Cases_on `p` THEN FULL_SIMP_TAC (srw_ss()) [subtree_def] THEN
 Cases_on `t0` THEN Cases_on `t1` THEN 
-FULL_SIMP_TAC (srw_ss()) [rootRep, root_def, isSubtree] THEN
-Cases_on `p` THEN FULL_SIMP_TAC (srw_ss()) [subtree]) THEN
+FULL_SIMP_TAC (srw_ss()) [rootRep_def, root_def, isSubtree_def] THEN
+Cases_on `p` THEN FULL_SIMP_TAC (srw_ss()) [subtree_def]) THEN
  
-`isSubtreeEq t1 (Node n l) ∧ rootRep t0 t1` by METIS_TAC [symRepProp] THEN
+`isSubtreeEq t1 (Node n l) ∧ rootRep t0 t1` by METIS_TAC [symRepProp_def] THEN
 FULL_SIMP_TAC (srw_ss()) [isSubEqImpSub] THEN
 SRW_TAC [][] THEN1
 
-(`(root t0 = NTS n) ∧ isSubtree t0 (Node n l)` by METIS_TAC [rootRep, root_def] THEN
-`height t0 < height (Node n l)` by METIS_TAC [subtreeHeight, isSubtree] THEN
+(`(root t0 = NTS n) ∧ isSubtree t0 (Node n l)` by METIS_TAC [rootRep_def, root_def] THEN
+`height t0 < height (Node n l)` by METIS_TAC [subtreeHeight, isSubtree_def] THEN
 Cases_on `∃s0 s1 t'.symRepProp s0 s1 t' ∧ isSubtree t' (Node n l)` THEN1
 
-(FULL_SIMP_TAC (srw_ss()) [symRepProp, rootRep, isSubEqImpSub] THEN
+(FULL_SIMP_TAC (srw_ss()) [symRepProp_def, rootRep_def, isSubEqImpSub] THEN
 SRW_TAC [][] THEN1
-(`height s1 < height (Node n l)` by METIS_TAC [subtreeHeight, isSubtree] THEN
+(`height s1 < height (Node n l)` by METIS_TAC [subtreeHeight, isSubtree_def] THEN
 `lastExpProp s1` by METIS_TAC [subtreeTrans] THEN
  METIS_TAC [subtreeLastExp]) THEN
-`height t' < height (Node n l)` by METIS_TAC [subtreeHeight, isSubtree] THEN
+`height t' < height (Node n l)` by METIS_TAC [subtreeHeight, isSubtree_def] THEN
 `lastExpProp t'` by METIS_TAC [subtreeTrans] THEN
  METIS_TAC [subtreeLastExp]) THEN
 
@@ -241,15 +78,15 @@ Q.EXISTS_TAC `t0` THEN
 Q.EXISTS_TAC `Node n l` THEN
 SRW_TAC [][] THEN
 `isSubtree e (Node n l)` by
-(SRW_TAC [][isSubtree] THEN
+(SRW_TAC [][isSubtree_def] THEN
 IMP_RES_TAC memImpEl THEN
 Q.EXISTS_TAC `[i]` THEN
-SRW_TAC [][subtree] THEN
-Cases_on `EL i l` THEN FULL_SIMP_TAC (srw_ss()) [subtree]) THEN
+SRW_TAC [][subtree_def] THEN
+Cases_on `EL i l` THEN FULL_SIMP_TAC (srw_ss()) [subtree_def]) THEN
 METIS_TAC []) THEN
 
-(`(root t0 = root t1) ∧ isSubtree t0 t1` by METIS_TAC [rootRep, root_def] THEN
-`height t1 < height (Node n l)` by METIS_TAC [subtreeHeight, isSubtree] THEN
+(`(root t0 = root t1) ∧ isSubtree t0 t1` by METIS_TAC [rootRep_def, root_def] THEN
+`height t1 < height (Node n l)` by METIS_TAC [subtreeHeight, isSubtree_def] THEN
 Cases_on `∃s0 s1.symRepProp s0 s1 t1 ∧ isSubtree t1 (Node n l)` THEN1
 
  (FULL_SIMP_TAC (srw_ss()) [] THEN
@@ -262,93 +99,17 @@ Q.EXISTS_TAC `t0` THEN
 Q.EXISTS_TAC `t1` THEN
 SRW_TAC [][] THEN
 Cases_on `t1` THEN1 
- (Cases_on `t0` THEN FULL_SIMP_TAC (srw_ss()) [root_def, rootRep, isSubtree] THEN
-  Cases_on `p'` THEN FULL_SIMP_TAC (srw_ss()) [subtree]) THEN
+ (Cases_on `t0` THEN FULL_SIMP_TAC (srw_ss()) [root_def, rootRep_def, isSubtree_def] THEN
+  Cases_on `p'` THEN FULL_SIMP_TAC (srw_ss()) [subtree_def]) THEN
 SRW_TAC [][] THEN
 IMP_RES_TAC memImpEl THEN
 `isSubtree e (Node n' l')` by
-(SRW_TAC [][isSubtree] THEN
+(SRW_TAC [][isSubtree_def] THEN
 Q.EXISTS_TAC `[i]` THEN
-SRW_TAC [][subtree] THEN
-Cases_on `EL i l'` THEN SRW_TAC [][subtree]) THEN
-METIS_TAC [subtreeNotSymProp, isSubtree]));
+SRW_TAC [][subtree_def] THEN
+Cases_on `EL i l'` THEN SRW_TAC [][subtree_def]) THEN
+METIS_TAC [subtreeNotSymProp, isSubtree_def]));
 
-
-val cnfTree = store_thm
-("cnfTree",
-``∀g tree. validptree g tree ⇒ isCnf g ⇒ ∀n t. (tree = Node n t) ⇒
-    ∃n1 t1 n2 t2.(t = [Node n1 t1; Node n2 t2]) ∨ ∃ts.(t = [Leaf ts])``,
-
-HO_MATCH_MP_TAC validptree_ind THEN SRW_TAC [][] THEN
-FULL_SIMP_TAC (srw_ss()) [validptree, isCnf_def] THEN
-RES_TAC THEN
-FULL_SIMP_TAC (srw_ss()) [list_lem2, list_lem1] THEN1
-(Cases_on `e1` THEN Cases_on `e2` THEN
- SRW_TAC [][] THEN
- FULL_SIMP_TAC (srw_ss()) [isNonTmnlSym_def, isNode_def] THEN1
-(`∃t1 t2.ptl = [Node n' t1; Node n'' t2]` by METIS_TAC [getSymsNtm] THEN
-METIS_TAC []) THEN
-(RES_TAC THEN
-FULL_SIMP_TAC (srw_ss()) [] THEN SRW_TAC [][] THEN
-FULL_SIMP_TAC (srw_ss()) [isNonTmnlSym_def])) THEN
-FULL_SIMP_TAC (srw_ss()) [] THEN
-RES_TAC THEN
-FULL_SIMP_TAC (srw_ss()) [] THEN SRW_TAC [][] THEN
-Cases_on `e` THEN FULL_SIMP_TAC (srw_ss()) [isTmnlSym_def] THEN
-`ptl = [Leaf t]` by METIS_TAC [getSymsTm] THEN
-METIS_TAC []);
-
-
-
-val treeSymsImpSubtree = store_thm
-("treeSymsImpSubtree",
-``∀t. e ∈ treeSyms t ⇒ ∃t1. isSubtreeEq t1 t ∧ (root t1 = e)``,
-
-completeInduct_on `height t` THEN SRW_TAC [][] THEN
-Cases_on `t` THEN FULL_SIMP_TAC (srw_ss()) [height_def, treeSyms] THEN1
-(SRW_TAC [][isSubtreeEq] THEN
-Q.EXISTS_TAC `Leaf t'` THEN
-SRW_TAC [][root_def] THEN
-Q.EXISTS_TAC `[]` THEN SRW_TAC [][subtree]) THEN1
-(SRW_TAC [][] THEN
-Q.EXISTS_TAC `Node n l` THEN
-SRW_TAC [][root_def, isSubtreeEq] THEN
-Q.EXISTS_TAC `[]` THEN SRW_TAC [][subtree]) THEN
-
-FULL_SIMP_TAC (srw_ss()) [MEM_FLAT, MEM_MAP] THEN
-SRW_TAC [][] THEN
-`isSubtree a (Node n l)` by
-(IMP_RES_TAC memImpEl THEN
-SRW_TAC [][isSubtree] THEN
-Q.EXISTS_TAC `[i']` THEN
-SRW_TAC [][subtree] THEN
-Cases_on `EL i' l`THEN SRW_TAC [][subtree]) THEN
-`height a < 1 + max 0 (MAP (λa. height a) l)` by
-(`height a < height (Node n l)`by METIS_TAC [subtreeHeight, isSubtree] THEN
-FULL_SIMP_TAC (srw_ss()) [height_def]) THEN
-METIS_TAC [subtreeTrans, isSubtree, isSubEqImpSub]);
-
-
-
-val notSymRepImpTreeSyms = store_thm
-("notSymRepImpTreeSyms",
-``(∀t0 t1. ¬symRepProp t0 t1 (Node n ptl)) ⇒ 
-(∀e. e ∈ ptl ⇒ ¬((NTS n) ∈ treeSyms e))``,
-
-SRW_TAC [][] THEN
-SPOSE_NOT_THEN ASSUME_TAC THEN
-IMP_RES_TAC treeSymsImpSubtree THEN
-`isSubtree e (Node n ptl)` by
-(IMP_RES_TAC memImpEl THEN
-SRW_TAC [][isSubtree] THEN
-Q.EXISTS_TAC `[i']` THEN
-SRW_TAC [][subtree] THEN
-Cases_on `EL i' ptl` THEN SRW_TAC [][subtree]) THEN
-
-`symRepProp t1 (Node n ptl) (Node n ptl)` by
-(FULL_SIMP_TAC (srw_ss()) [symRepProp, isSubEqImpSub, rootRep, root_def] THEN
-METIS_TAC [isSubtree, subtreeTrans]) THEN
-METIS_TAC []);
 
 
 val inpLen = store_thm
@@ -371,7 +132,7 @@ FULL_SIMP_TAC (srw_ss()) [validptree, height_def, isCnf_def] THEN
  Cases_on `e` THEN FULL_SIMP_TAC (srw_ss()) [isTmnlSym_def] THEN
  SRW_TAC [][leaves_def] THEN
  `l = [Leaf t]` by METIS_TAC [getSymsTm] THEN
- SRW_TAC [][leaves_def, distinctNtms, treeSyms, rmDupes, delete_def]) THEN
+ SRW_TAC [][leaves_def, distinctNtms_def, treeSyms_def, rmDupes, delete_def]) THEN
 
 FULL_SIMP_TAC (srw_ss()) [list_lem2] THEN
 Cases_on `e1` THEN Cases_on `e2` THEN SRW_TAC [][] THEN
@@ -389,8 +150,8 @@ Q.ABBREV_TAC `l = LENGTH (leaves t)` THEN
 Q.ABBREV_TAC `l1 = LENGTH (leaves t1)` THEN
 Q.ABBREV_TAC `l2 = LENGTH (leaves t2)` THEN
 
-`(subtree t [0] = SOME t1)` by SRW_TAC [][subtree, Abbr `t`, Abbr `t1`] THEN
-`(subtree t [1] = SOME t2)` by SRW_TAC [][subtree, Abbr `t`, Abbr `t2`] THEN
+`(subtree t [0] = SOME t1)` by SRW_TAC [][subtree_def, Abbr `t`, Abbr `t1`] THEN
+`(subtree t [1] = SOME t2)` by SRW_TAC [][subtree_def, Abbr `t`, Abbr `t2`] THEN
 `¬∃s0 s1. symRepProp s0 s1 t1` by METIS_TAC [subtreeNotSymProp, MEM] THEN
 `¬∃s0 s1. symRepProp s0 s1 t2` by METIS_TAC [subtreeNotSymProp, MEM] THEN
 
@@ -413,7 +174,7 @@ SRW_TAC [][] THEN
 `LENGTH d1 ≤ LENGTH d - 1` by
 
 (SRW_TAC [][Abbr `d1`, Abbr `d`, Abbr `t1`, Abbr `t`] THEN
-SRW_TAC [][distinctNtms] THEN
+SRW_TAC [][distinctNtms_def] THEN
 SRW_TAC [][rmDupes_lts_card] THEN
 Q.MATCH_ABBREV_TAC `CARD (set s0) ≤ CARD (set s) - 1` THEN
 Q_TAC SUFF_TAC `CARD (set s0) < CARD (set s)` THEN
@@ -421,7 +182,7 @@ FULL_SIMP_TAC (arith_ss) [] THEN
 Q_TAC SUFF_TAC `set s0 ⊂ set s` THEN1
  METIS_TAC [CARD_PSUBSET, FINITE_LIST_TO_SET] THEN
 UNABBREV_ALL_TAC THEN
-FULL_SIMP_TAC (srw_ss()) [treeSyms, rmDupes, delete_def, isNonTmnlSym_def] THEN
+FULL_SIMP_TAC (srw_ss()) [treeSyms_def, rmDupes, delete_def, isNonTmnlSym_def] THEN
 FULL_SIMP_TAC (srw_ss()) [FILTER_APPEND, isNonTmnlSym_def] THEN
 `delete (NTS n) (FILTER isNonTmnlSym (FLAT (MAP (λa. treeSyms a) t'))) =
 (FILTER isNonTmnlSym (FLAT (MAP (λa. treeSyms a) t')))`
@@ -439,7 +200,7 @@ METIS_TAC [rmd_r2, MEM, MEM_APPEND, delete_not_mem, delete_append,
 `LENGTH d2 ≤ LENGTH d - 1` by
 
 (SRW_TAC [][Abbr `d2`, Abbr `d`, Abbr `t2`, Abbr `t`] THEN
-SRW_TAC [][distinctNtms] THEN
+SRW_TAC [][distinctNtms_def] THEN
 SRW_TAC [][rmDupes_lts_card] THEN
 Q.MATCH_ABBREV_TAC `CARD (set s0) ≤ CARD (set s) - 1` THEN
 Q_TAC SUFF_TAC `CARD (set s0) < CARD (set s)` THEN
@@ -447,7 +208,7 @@ FULL_SIMP_TAC (arith_ss) [] THEN
 Q_TAC SUFF_TAC `set s0 ⊂ set s` THEN1
  METIS_TAC [CARD_PSUBSET, FINITE_LIST_TO_SET] THEN
 UNABBREV_ALL_TAC THEN
-FULL_SIMP_TAC (srw_ss()) [treeSyms, rmDupes, delete_def] THEN
+FULL_SIMP_TAC (srw_ss()) [treeSyms_def, rmDupes, delete_def] THEN
 FULL_SIMP_TAC (srw_ss()) [FILTER_APPEND, isNonTmnlSym_def] THEN
 `delete (NTS n) (FILTER isNonTmnlSym (FLAT (MAP (λa. treeSyms a) t''))) =
 (FILTER isNonTmnlSym (FLAT (MAP (λa. treeSyms a) t'')))`
@@ -469,8 +230,8 @@ METIS_TAC [rmd_r2, MEM, MEM_APPEND, delete_not_mem, delete_append,
 `l1 + l2 ≤ 2 ** (((LENGTH d - 1) - 1) + 1)` by METIS_TAC [powMult] THEN
 `LENGTH d ≥ 2` by
 (SRW_TAC [][Abbr `d`, Abbr `t`, Abbr `t1`, Abbr `t2`] THEN
-FULL_SIMP_TAC (srw_ss()) [treeSyms] THEN
-SRW_TAC [][distinctNtms, treeSyms, rmDupes, delete_def, delete_append,
+FULL_SIMP_TAC (srw_ss()) [treeSyms_def] THEN
+SRW_TAC [][distinctNtms_def, treeSyms_def, rmDupes, delete_def, delete_append,
 	   FILTER_APPEND, isNonTmnlSym_def] THEN
 DECIDE_TAC) THEN
 Cases_on `LENGTH d` THEN FULL_SIMP_TAC (srw_ss()) [] THEN
@@ -478,13 +239,7 @@ Cases_on `LENGTH d` THEN FULL_SIMP_TAC (srw_ss()) [] THEN
 FULL_SIMP_TAC (srw_ss()++ARITH_ss) []);
 
 
-val numd = store_thm
-("numd",
- ``∀t. isNode t ⇒ LENGTH (distinctNtms t) ≥ 1``,
 
-Cases_on `t` THEN SRW_TAC [][distinctNtms, treeSyms, rmDupes, delete_def,isNode_def,
-			     rmDupes, FILTER_APPEND, isNonTmnlSym_def] THEN
-DECIDE_TAC);
 
 val inpLeninv = store_thm
 ("inpLeninv",
@@ -500,379 +255,6 @@ Q.ABBREV_TAC `k = LENGTH (distinctNtms t)` THEN
 METIS_TAC [inpLen]);
 
 
-
-val subtreeLevel = store_thm
-("subtreeLevel",
-``∀t p. (subtree t p = SOME t1) ∧ p ≠ [] ⇒
-   ∃n ptl. (subtree t (FRONT p) = SOME (Node n ptl)) ∧ MEM t1 ptl``,
-
-Induct_on `p` THEN SRW_TAC [][] THEN
-Cases_on `t` THEN FULL_SIMP_TAC (srw_ss()) [subtree] THEN
-Cases_on `h < LENGTH l` THEN FULL_SIMP_TAC (srw_ss()) [] THEN
-Cases_on `p` THEN FULL_SIMP_TAC (srw_ss()) [] THEN1
-
-(Cases_on `EL h l` THEN
-FULL_SIMP_TAC (srw_ss()) [subtree] THEN
-SRW_TAC [][] THEN
-METIS_TAC [EL_IS_EL]) THEN
-SRW_TAC [][subtree]);
-
-
-val ntmsLen = store_thm
-("ntmsLen",
-``LENGTH (ntms g) ≥ 1``,
-
-Cases_on `g` THEN 
-SRW_TAC [][ntms_def, ntList_def, nonTerminalsList_def, startSym_def,
-	   rmDupes] THEN
-DECIDE_TAC);
-
-
-val distNtmsSub = store_thm
-("distNtmsSub",
-``∀g t. validptree g t ⇒ set (distinctNtms t) ⊆  set (MAP NTS (ntms g))``,
-
-HO_MATCH_MP_TAC validptree_ind THEN
-SRW_TAC [][validptree] THEN
-`∀e. e ∈ ptl ∧ isNode e ⇒ set (distinctNtms e) ⊆ set (MAP NTS (ntms g))`
-by METIS_TAC [] THEN
-`∀e. e ∈ ptl ⇒ set (distinctNtms e) ⊆ set (MAP NTS (ntms g))` by
-(SRW_TAC [][] THEN
-Cases_on `e` THEN1
-SRW_TAC [][distinctNtms, isNonTmnlSym_def, treeSyms, rmDupes, delete_def] THEN
-METIS_TAC [isNode_def]) THEN
-`n ∈ (ntms g)`  by METIS_TAC [ruleRhsInntms] THEN
-`((NTS n):(α,β) symbol) ∈ (MAP NTS (ntms g))`  by SRW_TAC [][MEM_MAP] THEN
-FULL_SIMP_TAC (srw_ss()) [distinctNtms, treeSyms, isNonTmnlSym_def,
-			  SUBSET_DEF, EXTENSION] THEN
-SRW_TAC [][] THEN
-FULL_SIMP_TAC (srw_ss())[rmDupes] THEN
-`x ∈ (FILTER isNonTmnlSym (FLAT (MAP (λa. treeSyms a) ptl)))`
- by METIS_TAC [memdel, rmd_r2] THEN
-FULL_SIMP_TAC (srw_ss()) [MEM_FILTER, MEM_MAP, MEM_FLAT] THEN
-SRW_TAC [][] THEN
-`x ∈ FILTER isNonTmnlSym (treeSyms a)` by METIS_TAC [MEM_FILTER] THEN
-Cases_on `x` THEN FULL_SIMP_TAC (srw_ss()) [isNonTmnlSym_def] THEN
-METIS_TAC [rmd_r2, symbol_11]);
-
-
-val LENGTH_distinctNtms = store_thm(
-  "LENGTH_distinctNtms",
-  ``LENGTH (distinctNtms t) = CARD (set (distinctNtms t))``,
-  SRW_TAC [][distinctNtms, rmDupes_lts_card, rmDupes_lts_card_eq]);
-
-val LENGTH_ntms = store_thm(
-  "LENGTH_ntms",
-  ``LENGTH (ntms t) = CARD (set (ntms t))``,
-  SRW_TAC [][ntms_def, rmDupes_lts_card, rmDupes_lts_card_eq]);
-
-
-val mapCard = store_thm
-("mapCard",
-``∀s. FINITE s ⇒ ∀l.(s = set l) ⇒ (∀x y.(f x = f y) ⇔ (x = y)) ⇒ 
- (CARD (set (MAP f l)) = CARD s)``,
-
-HO_MATCH_MP_TAC FINITE_INDUCT THEN SRW_TAC [][] THEN
-`∃l'. (set l' = s)` by  METIS_TAC [listExists4Set] THEN
-FIRST_X_ASSUM (Q.SPECL_THEN [`l'`] MP_TAC) THEN SRW_TAC [][] THEN
-`set l = e INSERT set l'` by METIS_TAC [] THEN
-FULL_SIMP_TAC (srw_ss()) [] THEN
-`¬(f e ∈ (MAP f l'))`  by FULL_SIMP_TAC (srw_ss()) [MEM_MAP] THEN
-`CARD ((f e) INSERT (set (MAP f l'))) = CARD (e INSERT set l')` by SRW_TAC [][] THEN
-`set (MAP f l) = f e INSERT set (MAP f l')` by
- (FULL_SIMP_TAC (srw_ss()) [EXTENSION] THEN
-  METIS_TAC [MEM_MAP]) THEN
-`CARD (e INSERT set l') = SUC (CARD (set l'))` 
- by FULL_SIMP_TAC (srw_ss()) [EXTENSION] THEN
-METIS_TAC []);
-
-
-val numdLeqNtms = store_thm
-("numdLeqNtms",
-``∀g t. validptree g t ⇒ LENGTH (distinctNtms t) ≤ LENGTH (ntms g)``,
-
-SRW_TAC [][] THEN
-Q_TAC SUFF_TAC ` LENGTH (distinctNtms t) ≤ 
- LENGTH ((MAP NTS (ntms g)):(α,β) symbol list)` THEN1
- METIS_TAC [LENGTH_MAP] THEN
-IMP_RES_TAC distNtmsSub THEN
-`FINITE (set (distinctNtms t))` by METIS_TAC [FINITE_LIST_TO_SET] THEN
-SRW_TAC [][LENGTH_ntms, LENGTH_distinctNtms] THEN
-`∀x y.(NTS x = NTS y) ⇔ (x = y)` by FULL_SIMP_TAC (srw_ss()) [] THEN
-`CARD (set ((MAP NTS (ntms g)):(α,β) symbol list)) =
-CARD (set (ntms g))` by METIS_TAC [mapCard, FINITE_LIST_TO_SET] THEN
-METIS_TAC [CARD_SUBSET, FINITE_LIST_TO_SET, DECIDE ``a ≤ b ∧b ≤ c ⇒ a ≤ c``]);
-
-val cleavesApp = store_thm
-("cleavesApp",
-``∀a b. cleaves (a ++ b) = cleaves a ++ cleaves b``,
-
-Induct_on `a` THEN SRW_TAC [][leaves_def]);
-
-
-val subtreePfxSfxLeaves = store_thm
-("subtreePfxSfxLeaves",
-``∀t t1 p.(subtree t p = SOME t1) ⇒ 
-∃pfx sfx.(leaves t = pfx ++ leaves t1 ++ sfx)``,
-
-Induct_on `p` THEN SRW_TAC [][] THEN1
-
-(Cases_on `t` THEN FULL_SIMP_TAC (srw_ss()) [subtree] THEN
- METIS_TAC [APPEND_NIL]) THEN
-
-Cases_on `t` THEN
-FULL_SIMP_TAC (srw_ss()) [] THEN1
-FULL_SIMP_TAC (srw_ss()) [subtree] THEN
-FULL_SIMP_TAC (srw_ss()) [subtree] THEN
-Cases_on `h < LENGTH l` THEN FULL_SIMP_TAC (srw_ss()) [] THEN
-FIRST_X_ASSUM (Q.SPECL_THEN [`EL h l`,`t1`] MP_TAC) THEN SRW_TAC [][] THEN
-
-(Cases_on `EL h l` THEN
-FULL_SIMP_TAC (srw_ss()) [subtree, leaves_def] THEN
-SRW_TAC [][leaves_def] THEN
-`MEM (EL h l) l` by METIS_TAC [EL_IS_EL] THEN
-FULL_SIMP_TAC (srw_ss()) [rgr_r9eq] THEN
-ONCE_ASM_REWRITE_TAC [] THEN
-SRW_TAC [][cleavesApp, leaves_def] THEN
-METIS_TAC [APPEND_ASSOC]));
-
-val cnfTreeLeaves = store_thm
-("cnfTreeLeaves",
-``∀g t. validptree g t ⇒ isCnf g ⇒ LENGTH (leaves t) ≥ 1``,
-
-HO_MATCH_MP_TAC validptree_ind THEN SRW_TAC [][] THEN
-FULL_SIMP_TAC (srw_ss()) [validptree, isCnf_def] THEN
-Q.ABBREV_TAC `r = getSymbols ptl` THEN
-`EVERY isNonTmnlSym r ∧ (LENGTH r = 2) ∨
-isWord r ∧ (LENGTH r = 1)` by METIS_TAC [] THEN
-SRW_TAC [][] THEN
-FULL_SIMP_TAC (srw_ss()) [list_lem2, list_lem1] THEN1
-(Cases_on `e1` THEN Cases_on `e2` THEN
- SRW_TAC [][] THEN
- FULL_SIMP_TAC (srw_ss()) [isNonTmnlSym_def, isNode_def] THEN
-`∃t1 t2.ptl = [Node n' t1; Node n'' t2]` by METIS_TAC [getSymsNtm] THEN
-SRW_TAC [][leaves_def] THEN
-FULL_SIMP_TAC (srw_ss()) [] THEN
-`LENGTH (leaves (Node n' t1)) ≥ 1`by METIS_TAC [isNode_def] THEN
-`LENGTH (leaves (Node n'' t2)) ≥ 1`by METIS_TAC [isNode_def] THEN
-FULL_SIMP_TAC (srw_ss()++ARITH_ss) [leaves_def]) THEN
-Cases_on `e` THEN
-SRW_TAC [][] THEN FULL_SIMP_TAC (srw_ss()) [isTmnlSym_def] THEN
-`(ptl = [Leaf t])` by METIS_TAC [getSymsTm] THEN
-SRW_TAC [][leaves_def]);
-
-
-
-val vptSubtree = store_thm
-("vptSubtree",
-``∀g t. validptree g t ⇒ 
- (∀t1. isSubtreeEq t1 t ∧ isNode t1 ⇒ validptree g t1)``,
-
-completeInduct_on `height t` THEN SRW_TAC [][] THEN
-Cases_on `t` THEN FULL_SIMP_TAC (srw_ss()) [] THEN1
-FULL_SIMP_TAC (srw_ss()) [validptree] THEN
-FULL_SIMP_TAC (srw_ss()) [isSubEqImpSub, isSubtree] THEN
-
-Cases_on `p` THEN FULL_SIMP_TAC (srw_ss()) [subtree] THEN
-Cases_on `h < LENGTH l` THEN FULL_SIMP_TAC (srw_ss()) [] THEN
-`isSubtreeEq t1 (EL h l)` by
-(SRW_TAC [][isSubEqImpSub, isSubtree] THEN
-Cases_on `t` THEN FULL_SIMP_TAC (srw_ss()) [subtree] THEN
-METIS_TAC [MEM]) THEN
-`isSubtree (EL h l) (Node n l)` by
-(SRW_TAC [][isSubtree] THEN
-Q.EXISTS_TAC `[h]` THEN SRW_TAC [][subtree] THEN
-Cases_on `EL h l` THEN SRW_TAC [][subtree]) THEN
-Cases_on `EL h l` THEN1
-(Cases_on `t` THEN FULL_SIMP_TAC (srw_ss()) [validptree, subtree] THEN
-Cases_on `t1` THEN FULL_SIMP_TAC (srw_ss()) [isNode_def]) THEN
-`height (EL h l) < height (Node n l)` by METIS_TAC [isSubtree, subtreeHeight] THEN
-FIRST_X_ASSUM (Q.SPECL_THEN [`height (EL h l)`] MP_TAC) THEN SRW_TAC [][] THEN
-FIRST_X_ASSUM (Q.SPECL_THEN [`EL h l`] MP_TAC) THEN SRW_TAC [][] THEN
-`validptree g (Node n' l')` by
-(FULL_SIMP_TAC (srw_ss()) [validptree] THEN
-METIS_TAC [isNode_def, EL_IS_EL, validptree]) THEN
-FIRST_X_ASSUM (Q.SPECL_THEN [`g`] MP_TAC) THEN SRW_TAC [][] THEN
-
-FULL_SIMP_TAC (srw_ss()) [isSubEqImpSub, isSubtree] THEN
-METIS_TAC []);
-
-
-
-val leafSubt = store_thm
-("leafSubt",
-``isSubtree t0 (Node n [Leaf ts]) ⇒ (t0 = Leaf ts)``,
-
-SRW_TAC [][isSubtree] THEN
-Cases_on `p` THEN FULL_SIMP_TAC (srw_ss()) [subtree] THEN
-Cases_on `h < 1` THEN FULL_SIMP_TAC (srw_ss()) [] THEN
-`h = 0` by DECIDE_TAC THEN
-SRW_TAC [][] THEN
-FULL_SIMP_TAC (srw_ss()) [] THEN
-Cases_on `t` THEN FULL_SIMP_TAC (srw_ss()) [subtree]);
-
-
-val subtDistNtms = store_thm
-("subtDistNtms",
-``∀t t1 p. (subtree t p = SOME t1) ⇒ 
-LENGTH (distinctNtms t1) ≤ LENGTH (distinctNtms t)``,
-
-Induct_on `p` THEN SRW_TAC [][] THEN
-Cases_on `t` THEN
-FULL_SIMP_TAC (srw_ss()) [subtree] THEN
-Cases_on `h < LENGTH l` THEN FULL_SIMP_TAC (srw_ss()) [] THEN
-FIRST_X_ASSUM (Q.SPECL_THEN [`EL h l`,`t1`] MP_TAC) THEN SRW_TAC [][] THEN
-
-`LENGTH (distinctNtms (EL h l)) ≤ LENGTH (distinctNtms (Node n l))`
-by (SRW_TAC [][distinctNtms, treeSyms] THEN
-`(EL h l) ∈ l`by METIS_TAC [EL_IS_EL] THEN
-FULL_SIMP_TAC (srw_ss()) [rgr_r9eq, isNonTmnlSym_def] THEN
-SRW_TAC [][] THEN
-Q_TAC SUFF_TAC `LENGTH (rmDupes (FILTER isNonTmnlSym (treeSyms (EL h l)))) ≤
-LENGTH
-  (rmDupes
-     (NTS n::
-          FILTER isNonTmnlSym
-            (FLAT (MAP (λa. treeSyms a) (r1 ++ [EL h l] ++ r2)))))` THEN1
-METIS_TAC [] THEN
-SRW_TAC [][FILTER_APPEND, FLAT_APPEND] THEN
-METIS_TAC [rmdLenLe, APPEND, APPEND_ASSOC]) THEN
-DECIDE_TAC);
-
-
-
-val distSymsLenSub = store_thm
-("distSymsLenSub",
-``∀t1 t. isSubtreeEq t1 t ⇒ LENGTH (distinctNtms t1) ≤ LENGTH (distinctNtms t)``,
-
-SRW_TAC [][isSubtreeEq] THEN
-METIS_TAC [subtDistNtms]);
-
-
-val getSymsCleaves = store_thm
-("getSymsCleaves",
-``∀g t. (∀e. e ∈ t ∧ isNode e ⇒ validptree g e) ⇒
-(derives g)^* (getSymbols t) (MAP TS (cleaves t))``,
-
-Induct_on `t` THEN SRW_TAC [][] THEN1
-SRW_TAC [][getSymbols_def, leaves_def] THEN
-Cases_on `h` THEN FULL_SIMP_TAC (srw_ss()) [getSymbols_def] THEN
-FULL_SIMP_TAC (srw_ss()) [cleavesApp, leaves_def] THEN1
-METIS_TAC [APPEND, rtc_derives_same_append_left, APPEND] THEN
-
-`(derives g)^* [NTS n] (MAP TS (leaves (Node n l)))`
- by METIS_TAC [vptRtcd, fringeEqLeaves, isNode_def, root_def] THEN
-FULL_SIMP_TAC (srw_ss()) [leaves_def] THEN
-METIS_TAC [APPEND, derives_append, APPEND]);
-
-
-val vptSubtD = store_thm
-("vptSubtD",
-``∀g t. validptree g t ⇒ ∀p t0. (subtree t p = SOME t0) ⇒
-∃pfx sfx. (derives g)^* [root t] (MAP TS pfx ++ [root t0] ++ MAP TS sfx) ∧
-(leaves t = pfx ++ leaves t0 ++ sfx)``,
-
-HO_MATCH_MP_TAC validptree_ind THEN SRW_TAC [][validptree] THEN
-Cases_on `p` THEN FULL_SIMP_TAC (srw_ss()) [subtree] THEN
-SRW_TAC [][] THEN1
-(MAP_EVERY Q.EXISTS_TAC [`[]`,`[]`] THEN
-SRW_TAC [][]) THEN
-
-Cases_on `h < LENGTH ptl` THEN FULL_SIMP_TAC (srw_ss()) [] THEN
-Cases_on `EL h ptl` THEN FULL_SIMP_TAC (srw_ss()) [] THEN1
-
-(Cases_on `t` THEN FULL_SIMP_TAC (srw_ss()) [subtree] THEN
-SRW_TAC [][] THEN
-IMP_RES_TAC EL_IS_EL THEN
-FULL_SIMP_TAC (srw_ss()) [rgr_r9eq, getSyms_append] THEN
-SRW_TAC [][] THEN
-ONCE_ASM_REWRITE_TAC [] THEN
-SRW_TAC [][root_def, leaves_def, cleavesApp] THEN
-`rule n (getSymbols (r1' ++ [Leaf t'] ++ r2')) ∈ rules g`
-by METIS_TAC [MEM, MEM_APPEND] THEN
-FULL_SIMP_TAC (srw_ss()) [getSyms_append, getSymbols_def] THEN
-MAP_EVERY Q.EXISTS_TAC [`cleaves r1'`,`cleaves r2'`]  THEN
-SRW_TAC [][] THEN
-`(derives g)^* (getSymbols r1') (MAP TS (cleaves r1'))`
-by METIS_TAC [getSymsCleaves, MEM, MEM_APPEND, validptree, rgr_r9eq] THEN
-`(derives g)^* (getSymbols r2') (MAP TS (cleaves r2'))`
-by METIS_TAC [getSymsCleaves, MEM, MEM_APPEND, validptree, rgr_r9eq] THEN
-
-`(derives g)^* ((getSymbols r1')++[TS t']) (MAP TS (cleaves r1') ++ [TS t'])`
-by METIS_TAC [rtc_derives_same_append_right] THEN
-`(derives g)^* ((getSymbols r1')++[TS t']++(getSymbols r1' ++ [TS t'])) 
-(MAP TS (cleaves r1') ++ [TS t']++(getSymbols r1' ++ [TS t']))`
-by METIS_TAC [rtc_derives_same_append_right] THEN
-`derives g [NTS n] (getSymbols r1' ++ [TS t'] ++ getSymbols r2')`
-by METIS_TAC [res1] THEN
-METIS_TAC [rtc_derives_same_append_left, rtc_derives_same_append_right,
-	   RTC_RULES, RTC_RTC]) THEN
-
-
-`isNode (EL h ptl)`by METIS_TAC [isNode_def] THEN
-Q.PAT_ASSUM `∀e. P e`MP_TAC THEN
-`Node n' l ∈ ptl` by METIS_TAC [EL_IS_EL] THEN
-FIRST_X_ASSUM (Q.SPECL_THEN [`EL h ptl`] MP_TAC) THEN SRW_TAC [][] THEN
-`∃pfx sfx. (derives g)^* [root (Node n' l)] 
-(MAP TS pfx ++ [root t0] ++ MAP TS sfx) ∧
-(leaves (Node n' l) = pfx ++ leaves t0 ++ sfx)`  by METIS_TAC [] THEN
-FULL_SIMP_TAC (srw_ss()) [leaves_def] THEN
-FULL_SIMP_TAC (srw_ss()) [rgr_r9eq] THEN
-SRW_TAC [][cleavesApp, leaves_def] THEN
-FULL_SIMP_TAC (srw_ss()) [root_def] THEN
-`rule n (getSymbols (r1' ++ [Node n' l] ++ r2'))∈ rules g`
-by METIS_TAC [MEM, MEM_APPEND] THEN
-MAP_EVERY Q.EXISTS_TAC [`cleaves r1'++pfx`,`sfx ++ cleaves r2'`] THEN
-SRW_TAC [][] THEN
-`(derives g)^* (getSymbols r1') (MAP TS (cleaves r1'))`
-by METIS_TAC [getSymsCleaves, MEM, MEM_APPEND, validptree, rgr_r9eq] THEN
-`(derives g)^* (getSymbols r2') (MAP TS (cleaves r2'))`
-by METIS_TAC [getSymsCleaves, MEM, MEM_APPEND, validptree, rgr_r9eq] THEN
-`derives g [NTS n] (getSymbols (r1' ++ [Node n' l] ++ r2'))`
-by METIS_TAC [res1] THEN
-FULL_SIMP_TAC (srw_ss()) [getSyms_append, getSymbols_def] THEN
-`(derives g)^* (getSymbols [Node n' l]) (MAP TS (cleaves [Node n' l]))`
-by METIS_TAC [getSymsCleaves, MEM, MEM_APPEND, validptree, rgr_r9eq] THEN
-FULL_SIMP_TAC (srw_ss()) [getSymbols_def, leaves_def] THEN
-`(derives g)^* ((getSymbols r1')++[NTS n']) (MAP TS (cleaves r1') ++ [NTS n'])`
-by METIS_TAC [rtc_derives_same_append_right] THEN
-`(derives g)^* (MAP TS (cleaves r1')++[NTS n']++getSymbols r2') 
-(MAP TS (cleaves r1') ++ [NTS n'] ++ getSymbols r2')`
-by METIS_TAC [rtc_derives_same_append_right, APPEND_ASSOC,RTC_RULES] THEN
-`(derives g)^* (MAP TS (cleaves r1') ++ [NTS n'] ++getSymbols r2') 
-(MAP TS (cleaves r1') ++ [NTS n'] ++MAP TS (cleaves r2'))`
-by METIS_TAC [rtc_derives_same_append_left, APPEND_ASSOC] THEN
-`(derives g)^* (MAP TS (cleaves r1') ++[NTS n'] ++ MAP TS (cleaves r2'))
-(MAP TS (cleaves r1') ++MAP TS pfx ++ [root t0] ++ MAP TS sfx ++ MAP TS (cleaves r2'))`
-by METIS_TAC [rtc_derives_same_append_left, rtc_derives_same_append_right,
-	      APPEND_ASSOC] THEN
-`(derives g)^* (getSymbols r1' ++ [NTS n'] ++ getSymbols r2')
-         (MAP TS (cleaves r1') ++ [NTS n'] ++ getSymbols r2')`
-by METIS_TAC [APPEND_ASSOC, rtc_derives_same_append_right] THEN
-METIS_TAC [APPEND_ASSOC, RTC_RTC, RTC_RULES]);
-
-val rtcDReplEnd = store_thm
-("rtcDReplEnd",
- ``∀i.(derives g)^* [NTS B] (p ++ [NTS B] ++ s) ∧
- (derives g)^*  [NTS B] z ∧ EVERY isTmnlSym z ∧
- (derives g)^* s z' ∧ EVERY isTmnlSym z'
-  ⇒
-  (derives g)^* [NTS B] (FLAT (lpow p i) ++ z ++ FLAT (lpow z' i))``,
-
-Induct_on `i` THEN SRW_TAC [][] THEN1
-(SRW_TAC [][lpow_def,REPLICATE] THEN
- METIS_TAC [rtc_derives_same_append_right,rtc_derives_same_append_left,
-	    APPEND_ASSOC,RTC_RTC]) THEN
-RES_TAC THEN
-SRW_TAC [][flatRepSuc] THEN
-Q_TAC SUFF_TAC
-`(derives g)^* [NTS B] (p ++ FLAT (lpow p i) ++ z ++  FLAT (lpow z' i) ++z')` THEN1
-METIS_TAC [flatRepComm,APPEND_ASSOC] THEN
-`(derives g)^* (p++[NTS B]++s) (p++FLAT (lpow p i) ++ z ++ FLAT (lpow z' i)++s)` by
-METIS_TAC [rtc_derives_same_append_right,rtc_derives_same_append_left,
-	   APPEND_ASSOC] THEN
-METIS_TAC [RTC_RTC,rtc_derives_same_append_left]);
-      
 
 val pumpCfg = store_thm
 ("pumpCfg",
@@ -907,13 +289,13 @@ Q.ABBREV_TAC `k0 = LENGTH (distinctNtms t)` THEN
 IMP_RES_TAC symPropImpLastExp THEN
 FULL_SIMP_TAC (srw_ss()) [lastExpProp] THEN
 SRW_TAC [][] THEN
-`validptree g (Node n ptl)` by METIS_TAC [symRepProp, vptSubtree, isNode_def] THEN
+`validptree g (Node n ptl)` by METIS_TAC [symRepProp_def, vptSubtree, isNode_def] THEN
 `isNode t0` by
-(Cases_on `t0` THEN FULL_SIMP_TAC (srw_ss()) [symRepProp, rootRep, root_def,
+(Cases_on `t0` THEN FULL_SIMP_TAC (srw_ss()) [symRepProp_def, rootRep_def, root_def,
 					     isNode_def]) THEN
-`validptree g (Node n ptl)` by METIS_TAC [symRepProp, vptSubtree, isNode_def] THEN
+`validptree g (Node n ptl)` by METIS_TAC [symRepProp_def, vptSubtree, isNode_def] THEN
 `validptree g t0` by 
-(FULL_SIMP_TAC (srw_ss()) [symRepProp, rootRep] THEN
+(FULL_SIMP_TAC (srw_ss()) [symRepProp_def, rootRep_def] THEN
  METIS_TAC [vptSubtree, isSubEqImpSub]) THEN
 
 `∃n1 n2 ptl1 ptl2. (ptl = [Node n1 ptl1; Node n2 ptl2])` by 
@@ -921,7 +303,7 @@ SRW_TAC [][] THEN
 by METIS_TAC [isNode_def, cnfTree] THEN1
 METIS_TAC [] THEN
 SRW_TAC [][] THEN
-FULL_SIMP_TAC (srw_ss()) [symRepProp, rootRep] THEN
+FULL_SIMP_TAC (srw_ss()) [symRepProp_def, rootRep_def] THEN
 `t0 = Leaf ts` by METIS_TAC [leafSubt] THEN
 SRW_TAC [][] THEN
 METIS_TAC [isNode_def]) THEN
@@ -937,15 +319,15 @@ Q.ABBREV_TAC `l2 = distinctNtms (Node n2 ptl2)` THEN
 `validptree g t2` by METIS_TAC [validptree, MEM, isNode_def] THEN
 `LENGTH (leaves t2) ≤ 2 ** (LENGTH l2 - 1)` by METIS_TAC [inpLen] THEN
 `∃p.(subtree (Node n [t1; t2]) p = SOME t0) ∧ p ≠ []`
-by  METIS_TAC [symRepProp, isSubtree, rootRep] THEN
+by  METIS_TAC [symRepProp_def, isSubtree_def, rootRep_def] THEN
 `∃p'. (subtree t p' = SOME (Node n [t1; t2]))` by  
-(FULL_SIMP_TAC (srw_ss()) [symRepProp] THEN
+(FULL_SIMP_TAC (srw_ss()) [symRepProp_def] THEN
  `((Node n [t1; t2]) = t) ∨ isSubtree (Node n [t1; t2]) t` 
  by METIS_TAC [isSubEqImpSub] THEN
  SRW_TAC [][] THEN
- METIS_TAC [subtree, isSubtree]) THEN
+ METIS_TAC [subtree_def, isSubtree_def]) THEN
 Cases_on `p` THEN FULL_SIMP_TAC (srw_ss()) [] THEN
-FULL_SIMP_TAC (srw_ss()) [subtree] THEN
+FULL_SIMP_TAC (srw_ss()) [subtree_def] THEN
 Cases_on `h < 2` THEN FULL_SIMP_TAC (srw_ss()) [] THEN
 `(h = 0) ∨ (h = 1)` by DECIDE_TAC THEN SRW_TAC [][]
 THENL[
@@ -967,17 +349,17 @@ THENL[
       SRW_TAC [][] THEN
       FULL_SIMP_TAC (arith_ss) [] THEN1      
       (`isSubtreeEq t1 t` by 
-      (FULL_SIMP_TAC (srw_ss())[isSubEqImpSub, symRepProp, isNode_def] THEN
-       SRW_TAC [][isSubtree] THEN
-       `(subtree (Node n [t1; t2]) [0] = SOME t1)` by SRW_TAC [][subtree] THEN
-       METIS_TAC [MEM, subtreeTrans, isSubtree]) THEN      
+      (FULL_SIMP_TAC (srw_ss())[isSubEqImpSub, symRepProp_def, isNode_def] THEN
+       SRW_TAC [][isSubtree_def] THEN
+       `(subtree (Node n [t1; t2]) [0] = SOME t1)` by SRW_TAC [][subtree_def] THEN
+       METIS_TAC [MEM, subtreeTrans, isSubtree_def]) THEN      
       `LENGTH l1 ≤ k0` by METIS_TAC [isSubEqImpSub, distSymsLenSub] THEN
       `LENGTH l1 ≤ k` by DECIDE_TAC THEN
       `isSubtreeEq t2 t` by 
-      (FULL_SIMP_TAC (srw_ss())[isSubEqImpSub, symRepProp, isNode_def] THEN
-       SRW_TAC [][isSubtree] THEN
-       `(subtree (Node n [t1; t2]) [1] = SOME t2)` by SRW_TAC [][subtree] THEN
-       METIS_TAC [MEM, subtreeTrans, isSubtree]) THEN      
+      (FULL_SIMP_TAC (srw_ss())[isSubEqImpSub, symRepProp_def, isNode_def] THEN
+       SRW_TAC [][isSubtree_def] THEN
+       `(subtree (Node n [t1; t2]) [1] = SOME t2)` by SRW_TAC [][subtree_def] THEN
+       METIS_TAC [MEM, subtreeTrans, isSubtree_def]) THEN      
       `LENGTH l2 ≤ k0` by METIS_TAC [isSubEqImpSub, distSymsLenSub] THEN
       `LENGTH l2 ≤ k` by DECIDE_TAC THEN       
       `LENGTH pfx' + (LENGTH sfx' + LENGTH (leaves t0)) ≤ 2 ** (k − 1)` 
@@ -999,7 +381,7 @@ THENL[
       METIS_TAC [vptRtcd,fringeEqLeaves] THEN
       `(derives g)^* [root t2] ((MAP TS (leaves t2)):(α,β) symbol list)` by
       METIS_TAC [vptRtcd,fringeEqLeaves] THEN
-      `root t0 = NTS n` by METIS_TAC [symRepProp, rootRep, root_def] THEN
+      `root t0 = NTS n` by METIS_TAC [symRepProp_def, rootRep_def, root_def] THEN
       `(derives g)^* [root t0] ((MAP TS (leaves t0)):(α,β) symbol list)` by
       METIS_TAC [vptRtcd,fringeEqLeaves] THEN
       Cases_on `t0` THEN FULL_SIMP_TAC (srw_ss()) [root_def] THEN
@@ -1011,7 +393,7 @@ THENL[
       
       `derives g [NTS n] [NTS n1;NTS n2]` by 
       (`isSubtreeEq (Node n [t1; t2]) t` by
-      (SRW_TAC [][isSubEqImpSub, isSubtree] THEN
+      (SRW_TAC [][isSubEqImpSub, isSubtree_def] THEN
       Cases_on `p'` THEN FULL_SIMP_TAC (srw_ss()) [] THEN
       METIS_TAC [MEM]) THEN
       `validptree g (Node n [t1;t2])` by METIS_TAC [isNode_def,vptSubtree] THEN
@@ -1063,17 +445,17 @@ THENL[
       SRW_TAC [][] THEN
       FULL_SIMP_TAC (arith_ss) [] THEN1      
       (`isSubtreeEq t2 t` by 
-      (FULL_SIMP_TAC (srw_ss())[isSubEqImpSub, symRepProp, isNode_def] THEN
-       SRW_TAC [][isSubtree] THEN
-       `(subtree (Node n [t1; t2]) [1] = SOME t2)` by SRW_TAC [][subtree] THEN
-       METIS_TAC [MEM, subtreeTrans, isSubtree]) THEN      
+      (FULL_SIMP_TAC (srw_ss())[isSubEqImpSub, symRepProp_def, isNode_def] THEN
+       SRW_TAC [][isSubtree_def] THEN
+       `(subtree (Node n [t1; t2]) [1] = SOME t2)` by SRW_TAC [][subtree_def] THEN
+       METIS_TAC [MEM, subtreeTrans, isSubtree_def]) THEN      
        `LENGTH l2 ≤ k0` by METIS_TAC [isSubEqImpSub, distSymsLenSub] THEN
       `LENGTH l2 ≤ k` by DECIDE_TAC THEN
       `isSubtreeEq t1 t` by 
-      (FULL_SIMP_TAC (srw_ss())[isSubEqImpSub, symRepProp, isNode_def] THEN
-       SRW_TAC [][isSubtree] THEN
-       `(subtree (Node n [t1; t2]) [0] = SOME t1)` by SRW_TAC [][subtree] THEN
-       METIS_TAC [MEM, subtreeTrans, isSubtree]) THEN      
+      (FULL_SIMP_TAC (srw_ss())[isSubEqImpSub, symRepProp_def, isNode_def] THEN
+       SRW_TAC [][isSubtree_def] THEN
+       `(subtree (Node n [t1; t2]) [0] = SOME t1)` by SRW_TAC [][subtree_def] THEN
+       METIS_TAC [MEM, subtreeTrans, isSubtree_def]) THEN      
       `LENGTH l1 ≤ k0` by METIS_TAC [isSubEqImpSub, distSymsLenSub] THEN
       `LENGTH l1 ≤ k` by DECIDE_TAC THEN       
       `LENGTH pfx' + (LENGTH sfx' + LENGTH (leaves t0)) ≤ 2 ** (k − 1)` 
@@ -1095,7 +477,7 @@ THENL[
       METIS_TAC [vptRtcd,fringeEqLeaves] THEN
       `(derives g)^* [root t2] ((MAP TS (leaves t2)):(α,β) symbol list)` by
       METIS_TAC [vptRtcd,fringeEqLeaves] THEN
-      `root t0 = NTS n` by METIS_TAC [symRepProp, rootRep, root_def] THEN
+      `root t0 = NTS n` by METIS_TAC [symRepProp_def, rootRep_def, root_def] THEN
       `(derives g)^* [root t0] ((MAP TS (leaves t0)):(α,β) symbol list)` by
       METIS_TAC [vptRtcd,fringeEqLeaves] THEN
       Cases_on `t0` THEN FULL_SIMP_TAC (srw_ss()) [root_def] THEN
@@ -1107,7 +489,7 @@ THENL[
       
       `derives g [NTS n] [NTS n1;NTS n2]` by 
       (`isSubtreeEq (Node n [t1; t2]) t` by
-      (SRW_TAC [][isSubEqImpSub, isSubtree] THEN
+      (SRW_TAC [][isSubEqImpSub, isSubtree_def] THEN
       Cases_on `p'` THEN FULL_SIMP_TAC (srw_ss()) [] THEN
       METIS_TAC [MEM]) THEN
       `validptree g (Node n [t1;t2])` by METIS_TAC [isNode_def,vptSubtree] THEN
