cfg-list/reachGenGrammarScript.sml
@@ -7,6 +7,15 @@ generatingGrammarTheory;
 val _ = new_theory "reachGenGrammar";
 
 
+val thm4_2Final = store_thm ("thm4_2Final",
+``language g ≠ {} ⇒ 
+∃g' g''. rgr g g' ∧ usefulnts g' g'' ∧ (language g = language g'')``,
+
+SRW_TAC [][] THEN
+`∃g'. rgr g g'` by METIS_TAC [rgr_exists] THEN
+`∃g''. usefulnts g' g''` by METIS_TAC [use_exists] THEN
+METIS_TAC [thm4_2, lemma4_1a]);
+
 val rugr = Define `rugr g g' = 
     ∃g0. usefulnts g g0 ∧
     (set (rules g') =
